rif/noninterference.v
@@ -1,0 +1,173 @@
+From mathcomp Require Import
+  ssreflect ssrfun ssrbool ssrnat eqtype seq choice fintype finfun.
+From CoqUtils Require Import hseq ord fset partmap word.
+From MicroPolicies Require Import
+  lib.utils lib.partmap_utils common.types rif.common rif.abstract.
+
+Set Implicit Arguments.
+Unset Strict Implicit.
+Unset Printing Implicit Defensive.
+
+Section Noninterference.
+
+Import DoNotation.
+
+Local Open Scope rif_scope.
+
+Variable Σ : finType.
+Variable mt : machine_types.
+Variable mops : machine_ops mt.
+Variable r_arg : reg mt.
+Variable output_addr : mword mt.
+Variable reclassify_addr : mword mt.
+
+Local Notation rifAutomaton := (rifAutomaton Σ).
+Local Notation rifLabel := (rifLabel Σ).
+Local Notation event := (event Σ mt).
+Local Notation ainstr := (ainstr Σ mt).
+Local Notation atom := (atom (mword mt) rifLabel).
+Local Notation state := (state Σ mt).
+Local Notation step := (@step Σ mt mops r_arg output_addr reclassify_addr).
+Local Notation stepn := (@stepn Σ mt mops r_arg output_addr reclassify_addr).
+
+Implicit Type st : state.
+
+CoInductive s_indist rs st1 st2 : Prop :=
+| SIndistLow of rl_readers (taga (pc st1)) ⊑ᵣ rs
+             &  pc st1 = pc st2
+             &  pointwise (indist (@rl_readers _ \o taga) rs)
+                          (regs st1) (regs st2)
+             &  pointwise (indist (fun t =>
+                                     if t is inr t'
+                                     then rl_readers (taga t')
+                                     else Anybody) rs)
+                          (mem st1) (mem st2)
+| SIndistHigh of ~~ (rl_readers (taga (pc st1)) ⊑ᵣ rs)
+              &  ~~ (rl_readers (taga (pc st2)) ⊑ᵣ rs).
+
+Ltac match_upd t1 :=
+  match goal with
+  | ind : pointwise ?P t1 ?t2,
+    upd : updm t1 ?x ?v1 = Some ?t1'
+    |- context[updm ?t2 ?x ?v2] =>
+    have: P v1 v2; last move=> /(refine_upd_pointwiseL ind upd)
+  end.
+
+Lemma low_step rs st1 st2 st1' oe1 :
+  s_indist rs st1 st2 ->
+  rl_readers (taga (pc st1)) ⊑ᵣ rs ->
+  step st1 = Some (st1', oe1) ->
+  match step st2 with
+  | Some (st2', oe2) =>
+    match oe1, oe2 with
+    | Some (Output w1 rs1), Some (Output w2 rs2) =>
+      indist (@snd _ _) rs (w1, rs1) (w2, rs2)
+      /\ s_indist rs st1' st2'
+    | Some (Reclassify rl1 F1), Some (Reclassify rl2 F2) =>
+      (rl1 == rl2) && (F1 == F2)
+    | None, None => s_indist rs st1' st2'
+    | _, _ => False
+    end
+  | None => False
+  end.
+Proof.
+move=> h_indist h_low1; case: h_indist; last by rewrite h_low1.
+rewrite (lock step).
+case: st1 {h_low1} => mem1 reg1 [pc1 rl1] oF1 /=.
+case: st2=> mem2 reg2 [pc2 rl2] oF2 /= h_pc e.
+move: pc1 rl1 e h_pc => pc rl [<- <-] h_pc {pc2 rl2} ind_r ind_m.
+rewrite -{1}lock /=.
+move: (ind_m pc).
+case get_pc1: (mem1 pc) => [[i1|a1]|] //=;
+case get_pc2: (mem2 pc) => [[i2|a2]|] //=;
+rewrite /indist /=.
+  (* Instructions *)
+  move=> e; move: i1 e get_pc1 get_pc2 => i /eqP [<-] {i2}.
+  case: i=> //=.
+  - (* Nop *)
+    move=> get_pc1 get_pc2 [<- <-] {st1' oe1}.
+    by rewrite -lock /= get_pc2; constructor.
+  - (* Const *)
+    move=> k r get_pc1 get_pc2.
+    case upd1: updm=> [reg1'|] //= [<- <-] {st1' oe1}.
+    rewrite -lock /= get_pc2.
+    match_upd reg1; first exact: indist_refl.
+    case=> reg2' [upd2 ind_r'].
+    by rewrite upd2 /=; constructor.
+  - (* Mov *)
+    move=> r1 r2 get_pc1 get_pc2.
+    move: (ind_r r1).
+    case get1: (reg1 r1) => [v1|] //=.
+    case get2: (reg2 r1) => [v2|] //= ind_v.
+    case upd1: (updm reg1) => [reg1'|] //= [<- <-] {st1' oe1}.
+    rewrite -lock /= get_pc2 get2 /=.
+    match_upd reg1=> // - [reg2' [upd2 ind_r']].
+    by rewrite upd2 /=; constructor.
+  - (* Binop *)
+    move=> b r1 r2 r3 get_pc1 get_pc2.
+    move: (ind_r r1).
+    case get11: (reg1 r1) => [[v11 l11]|] //=.
+    case get12: (reg2 r1) => [[v12 l12]|] //= ind_v1.
+    move: (ind_r r2).
+    case get21: (reg1 r2) => [[v21 l21]|] //=.
+    case get22: (reg2 r2) => [[v22 l22]|] //= ind_v2.
+    case upd1: updm=> [reg1'|] //= [<- <-] {st1' oe1}.
+    rewrite -lock /= get_pc2 get12 get22 /=.
+    match_upd reg1=> //=.
+      move: ind_v1 ind_v2; rewrite /indist /= !rl_readers_join !readers_join_min.
+      by repeat match goal with
+      | |- context[_ ⊑ᵣ _] => case: readers_leq=> //=
+      end; move=> /eqP [-> ->] /eqP [-> ->].
+    case=> regs2' [upd2 ind_r'].
+    by rewrite upd2 /=; constructor.
+  - (* Load *)
+    move=> r1 r2 get_pc1 get_pc2.
+    move: (ind_r r1).
+    case get_r1: (reg1 r1) => [[v1 l1]|] //=.
+    case get_r2: (reg2 r1) => [[v2 l2]|] //= ind_v.
+    move: (ind_m v1).
+    admit.
+  - (* Store *)
+    move=> r1 r2 get_pc1 get_pc2.
+    move: (ind_r r1).
+    case get_r11: (reg1 r1) => [[v11 l11]|] //=.
+    case get_r12: (reg2 r1) => [[v12 l12]|] //= ind_v1.
+    move: (ind_r r2).
+    case get_r21: (reg1 r2) => [[v21 l21]|] //=.
+    case get_r22: (reg2 r2) => [[v22 l22]|] //= ind_v2.
+    admit.
+  - (* Jump *)
+    move=> r get_pc1 get_pc2.
+    move: (ind_r r).
+    case get_r1: (reg1 r) => [[v1 l1]|] //=.
+    case get_r2: (reg2 r) => [[v2 l2]|] //= ind_v [<- <-] {st1' oe1}.
+    rewrite -lock /= get_pc2 get_r2 /=.
+    case/indistP: ind_v=> /= [lo1 lo2 [<- <-]|hi1 hi2].
+      constructor=> //=.
+      by rewrite rl_readers_join readers_join_min lo1.
+    by apply: SIndistHigh=> //=;
+    rewrite rl_readers_join readers_join_min negb_and ?hi1 ?hi2.
+  - (* Bnz *)
+    move=> r i get_pc1 get_pc2.
+    move: (ind_r r).
+    case get_r1: (reg1 r) => [[v1 l1]|] //=.
+    case get_r2: (reg2 r) => [[v2 l2]|] //= ind_v [<- <-] {st1' oe1}.
+    rewrite -lock /= get_pc2 get_r2 /=.
+    case/indistP: ind_v=> /= [lo1 lo2 [<- <-]|hi1 hi2].
+      constructor=> //=.
+      by rewrite rl_readers_join readers_join_min lo1.
+    by apply: SIndistHigh=> //=;
+    rewrite rl_readers_join readers_join_min negb_and ?hi1 ?hi2.
+  (* Jal *)
+  move=> r oF get_pc1 get_pc2.
+  move: (ind_r r).
+  case get_r1: (reg1 r) => [[v1 l1]|] //=.
+  case get_r2: (reg2 r) => [[v2 l2]|] //= ind_v.
+  case upd1: updm => [reg1'|] //= [<- <-] {st1' oe1}.
+  rewrite -lock /= get_pc2 get_r2 /=.
+  admit.
+(* System services *)
+admit.
+Admitted.
+
+End Noninterference.
